check_gameover.dfy
@@ -1,0 +1,52 @@
+include "board.dfy"
+
+
+
+method CanCaptureKing(possilbe_capture: Move, king_rank: int, king_file: int, piece: Piece, board: Board) returns (kill_king: bool)
+  requires possilbe_capture.PieceMove?
+  requires board.move_in_range(possilbe_capture)
+  requires possilbe_capture.capture 
+  requires board.CapturePre(possilbe_capture)
+{
+  match piece
+  case Pawn => 
+    return board.PawnPre(possilbe_capture);
+  case Rook =>
+  case Knight =>
+  case Bishop =>
+  case Queen =>
+  case King =>
+}
+
+method CheckChecker(king_color: Color, king_rank: int, king_file: int, board: Board) returns (check: bool)
+  requires 0 <= king_rank < 8 && 0 <= king_file < 8
+  requires board.grid.Length0 == board.grid.Length1 == 8
+{
+  var moves := new (int, int)[64](i => (-1, -1));
+  var idx := 0;
+  
+  for i := 0 to board.grid.Length0
+  {
+    for j := 0 to board.grid.Length1
+    {
+      if board.grid[i, j] == Empty {
+        continue;
+      }
+      if board.grid[i, j].color != king_color {
+        var possilbe_capture := PieceMove((i, j), (king_rank, king_file), capture := true);
+        check := CanCaptureKing(possilbe_capture, king_rank, king_file, board.grid[i, j].piece, board);
+        if check {
+          return;
+        }
+      }
+    }
+  }
+  
+  return false;
+}
+
+method Test() 
+{
+  var board := new Board();
+
+}
